gluing.lean
@@ -1,0 +1,159 @@
+import tactic
+import .topology
+noncomputable theory
+
+section covers
+
+-- cover of a set
+structure cover (I X : Type) :=
+  (part : I → set X)
+  (hx : ∀ (x : X), ∃ (i : I), x ∈ part i)
+
+-- consistent functions on each part of the cover
+structure gluing_data (I X Y : Type) :=
+  (U : cover I X)
+  (f : Π (i : I), (U.part i) → Y)
+  (hglue : ∀ (i j : I) (x : X) (hxi : x ∈ U.part i) (hxj : x ∈ U.part j),
+    (f i) ⟨x, hxi⟩ = (f j) ⟨x, hxj⟩)
+
+-- what it means for f : X → Y to be compatible with gluing data
+def compatible {I X Y : Type} (gldata : gluing_data I X Y) (f : X → Y) :=
+  ∀ (i : I) (x : X) (hxi : x ∈ gldata.U.part i), f x = gldata.f i ⟨x, hxi⟩
+
+lemma compatible_iff_restrict_eq
+  {I X Y : Type} (gldata : gluing_data I X Y) {f : X → Y} :
+  compatible gldata f ↔ ∀ (i : I), subtype.restrict f _ = gldata.f i :=
+begin
+  split; intros hf i, specialize hf i,
+  ext ⟨x, hx⟩, rw subtype.restrict_apply, exact hf x hx,
+  intros x hx, rw ← hf, rw subtype.restrict_apply,
+end
+
+-- existence of compatible function
+-- (uses choice, even though the result is unique)
+def mk_function {I X Y : Type} (gldata : gluing_data I X Y) : X → Y :=
+λ x, let ⟨i, hxi⟩ := classical.subtype_of_exists (gldata.U.hx x) in
+  gldata.f i ⟨x, hxi⟩
+
+lemma mk_compatible {I X Y} (gldata : @gluing_data I X Y) :
+  compatible gldata (mk_function gldata) :=
+begin
+  intros i x hxi,
+  let j := classical.subtype_of_exists (gldata.U.hx x),
+  exact gldata.hglue j.val i x j.prop hxi,
+end
+
+lemma compatible_unique {I X Y : Type} (gldata : @gluing_data I X Y) (f g : X → Y) :
+  compatible gldata f → compatible gldata g → f = g :=
+begin
+  intros hf hg,
+  ext, obtain ⟨i, hxi⟩ := gldata.U.hx x,
+  specialize hf i x hxi,
+  specialize hg i x hxi,
+  rwa [hf, hg],
+end
+
+section refine
+
+variables
+  (I J X Y : Type)
+  (CI : cover I X)
+  (CJ : cover J X)
+  (gldata : gluing_data I X Y)
+
+def refine : cover (I × J) X :=
+ ⟨λ ⟨i, j⟩, (CI.part i) ∩ (CJ.part j),
+  λ x, let ⟨i, hxi⟩ := CI.hx x in
+       let ⟨j, hxj⟩ := CJ.hx x in
+       ⟨⟨i, j⟩, ⟨hxi, hxj⟩⟩⟩
+
+/- 
+Note: this is asymmetric: f is defined on Uᵢ ∩ Vⱼ 
+as the restriction of f from Uᵢ, not Vⱼ.
+-/
+def gl_refine : gluing_data (I × J) X Y :=
+  ⟨ -- U, f, hglue
+    refine I J X gldata.U CJ, -- U
+    λ ⟨i, j⟩ ⟨x, hxij⟩,
+    gldata.f i ⟨x, hxij.left⟩,
+    λ ⟨i₁, j₁⟩ ⟨i₂, j₂⟩ x ⟨hxi₁, hxj₁⟩ ⟨hxi₂, hxj₂⟩,
+    gldata.hglue i₁ i₂ x hxi₁ hxi₂,
+  ⟩
+
+variable (f : X → Y)
+
+lemma compat_of_refine_of_compat :
+  compatible gldata f →
+  compatible (gl_refine _ _ _ _ CJ gldata) f :=
+begin
+  rintros hf ⟨i, j⟩ x ⟨hxi, hxj⟩,
+  exact hf i x hxi,
+end
+
+end refine
+
+end covers
+
+section open_cover
+
+open topology
+
+variables (I X Y : Type) (TX : topology X) (TY : topology Y)
+
+structure open_cover extends (cover I X) :=
+  (hopen : ∀ (i : I), part i ∈ TX.opens)
+
+instance : has_coe (open_cover I X TX) (cover I X) := ⟨λ U, ⟨U.part, U.hx⟩⟩
+
+structure cts_gluing_data :=
+  (U : open_cover I X TX)
+  (f : Π (i : I), (U.part i) → Y)
+  (hglue : ∀ (i j : I) (x : X) (hxi : x ∈ U.part i) (hxj : x ∈ U.part j),
+    (f i) ⟨x, hxi⟩ = (f j) ⟨x, hxj⟩)
+  (hf : Π (i : I), @cts _ _ (topology.subspace_topology TX (U.part i)) TY (f i))
+
+instance : has_coe (cts_gluing_data I X Y TX TY) (gluing_data I X Y) :=
+  ⟨λ gldata, ⟨gldata.U, gldata.f, gldata.hglue⟩⟩
+
+variables
+  (U : open_cover I X TX) (gldata : cts_gluing_data I X Y TX TY)
+  (f g : X → Y)
+
+lemma cts_iff_cts_on_cover (f : X → Y) : cts TX TY f ↔ 
+  Π (i : I), @cts _ _ (topology.subspace_topology TX (U.part i)) TY
+                      (subtype.restrict f _) :=
+begin
+  split,
+  intros hf i, apply pullback_cts_along_inverse_image, exact hf,
+  intro hfi,
+  -- check continuity pointwise, then on a piece of the cover
+  rw cts_iff_ptwise_cts, intro x,
+  obtain ⟨i, hxi⟩ := U.hx x, specialize hfi i,
+  rw cts_iff_ptwise_cts at hfi, specialize hfi ⟨x, hxi⟩,
+  rwa cts_at_pt_of_open TX TY f (U.part i) (U.hopen i) x hxi,
+end
+
+-- function compatible with cts gluing data is cts
+-- (mostly equivalent to cts_iff_cts_on_cover)
+lemma cts_of_cts_compat :
+  compatible (gldata : gluing_data I X Y) f → cts TX TY f :=
+begin
+  intro hf,
+  rw cts_iff_cts_on_cover I X Y TX TY gldata.U,
+  rw compatible_iff_restrict_eq at hf,
+  intro i, specialize hf i, convert gldata.hf i,
+end
+
+-- the glued function is continuous! 🎉
+lemma mk_function_cts : cts TX TY (mk_function (gldata : gluing_data I X Y)) :=
+  @cts_of_cts_compat I X Y TX TY gldata
+  (mk_function (gldata : gluing_data I X Y))
+  (mk_compatible ↑gldata)
+
+section fiber_bundle
+
+parameters 
+
+end fiber_bundle
+
+end open_cover
